theories/modules/LMod.v
@@ -2,19 +2,22 @@ From CRIS.common Require Export Common Fn.
 From CRIS.modules Require Export LModTr.
 
 Module LMod.
-  Record t : Type := mk {
-    fnsems : gmap fname (Any.t → itree lmodE Any.t);
-    initial_st : lstateT;
+  Record t (Σ : Type) : Type := mk {
+    fnsems : gmap fname (Any.t → itree (lmodE Σ) Any.t);
+    initial_st : lstateT Σ;
   }.
+
+  Arguments fnsems {Σ} _.
+  Arguments initial_st {Σ} _.
 
   (* Record wf (ms : t) : Prop := mk_wf {
     wf_fnsems : map_Forall (const is_Some) (fnsems ms);
   }. *)
 
-  Definition prog (ms : t) : string → option (Any.t → itree lmodE Any.t) :=
+  Definition prog {Σ} (ms : t Σ) : string → option (Any.t → itree (lmodE Σ) Any.t) :=
     λ fn, (fnsems ms) !! (funid fn).
 
-  Definition compile (ms : t) : Any.t → itree coreE Any.t := λ arg,
+  Definition compile {Σ} (ms : t Σ) : Any.t → itree coreE Any.t := λ arg,
     bd <- ((fnsems ms) !! entry)? ;;
     snd <$> LModTr.trans (prog ms) (bd arg) (initial_st ms).
 End LMod.
